barrier/lifting.v
@@ -2,7 +2,8 @@ Require Import prelude.gmap iris.lifting.
 Require Export iris.weakestpre barrier.heap_lang_tactics.
 Import uPred.
 Import heap_lang.
-Local Hint Extern 0 (reducible _ _) => do_step ltac:(eauto 2).
+Local Hint Extern 0 (language.reducible _ _) => do_step ltac:(eauto 2).
+Local Hint Extern 0 (head_reducible _ _) => do_step ltac:(eauto 2).
 
 Section lifting.
 Context {Σ : iFunctor}.
@@ -16,84 +17,75 @@ Lemma wp_bind {E e} K Q :
 Proof. apply wp_bind. Qed.
 
 (** Base axioms for core primitives of the language: Stateful reductions. *)
-Lemma wp_lift_step E1 E2 (φ : expr → state → Prop) Q e1 σ1 :
-  E1 ⊆ E2 → to_val e1 = None →
-  reducible e1 σ1 →
-  (∀ e2 σ2 ef, prim_step e1 σ1 e2 σ2 ef → ef = None ∧ φ e2 σ2) →
-  pvs E2 E1 (ownP σ1 ★ ▷ ∀ e2 σ2, (■ φ e2 σ2 ∧ ownP σ2) -★
-    pvs E1 E2 (wp E2 e2 Q))
-  ⊑ wp E2 e1 Q.
-Proof.
-  intros ? He Hsafe Hstep.
-  rewrite -(wp_lift_step E1 E2 (λ e' σ' ef, ef = None ∧ φ e' σ') _ _ σ1) //.
-  apply pvs_mono, sep_mono, later_mono; first done.
-  apply forall_mono=>e2; apply forall_mono=>σ2.
-  apply forall_intro=>ef; apply wand_intro_l.
-  rewrite always_and_sep_l' -associative -always_and_sep_l'.
-  apply const_elim_l=>-[-> ?] /=.
-  by rewrite const_equiv // left_id wand_elim_r right_id.
-Qed.
-
-(* TODO RJ: Figure out some better way to make the
-   postcondition a predicate over a *location* *)
 Lemma wp_alloc_pst E σ e v Q :
   to_val e = Some v →
   (ownP σ ★ ▷ (∀ l, ■(σ !! l = None) ∧ ownP (<[l:=v]>σ) -★ Q (LocV l)))
        ⊑ wp E (Alloc e) Q.
 Proof.
-  intros; set (φ e' σ' := ∃ l, e' = Loc l ∧ σ' = <[l:=v]>σ ∧ σ !! l = None).
-  rewrite -(wp_lift_step E E φ _ _  σ) // /φ; last by intros; inv_step; eauto.
+  intros; set (φ e' σ' ef := ∃ l, e' = Loc l ∧ σ' = <[l:=v]>σ ∧ σ !! l = None
+                                ∧ ef = (None : option expr)).
+  rewrite -(wp_lift_step E E φ _ _  σ) // /φ; last (by intros; inv_step; eauto); [].
   rewrite -pvs_intro. apply sep_mono, later_mono; first done.
-  apply forall_intro=>e2; apply forall_intro=>σ2; apply wand_intro_l.
+  apply forall_intro=>e2; apply forall_intro=>σ2; apply forall_intro=>ef.
+  apply wand_intro_l.
   rewrite -pvs_intro always_and_sep_l' -associative -always_and_sep_l'.
-  apply const_elim_l=>-[l [-> [-> ?]]].
-  by rewrite (forall_elim l) const_equiv // left_id wand_elim_r -wp_value'.
+  apply const_elim_l=>-[l [-> [-> [? ->]]]].
+  rewrite right_id (forall_elim l) const_equiv //.
+  by rewrite left_id wand_elim_r -wp_value'.
 Qed.
+
+Lemma wp_lift_atomic_det_step {E Q e1} σ1 v2 σ2 :
+  to_val e1 = None →
+  head_reducible e1 σ1 →
+  (∀ e' σ' ef, head_step e1 σ1 e' σ' ef → ef = None ∧ e' = of_val v2 ∧ σ' = σ2) →
+  (ownP σ1 ★ ▷ (ownP σ2 -★ Q v2)) ⊑ wp E e1 Q.
+Proof.
+  intros He Hsafe Hstep.
+  rewrite -(wp_lift_step E E (λ e' σ' ef, ef = None ∧ e' = of_val v2 ∧ σ' = σ2) _ e1 σ1) //; last first. 
+  { intros. by apply Hstep, prim_head_step. }
+  { by apply head_reducible_reducible. }
+  rewrite -pvs_intro. apply sep_mono, later_mono; first done.
+  apply forall_intro=>e2'; apply forall_intro=>σ2'.
+  apply forall_intro=>ef; apply wand_intro_l.
+  rewrite always_and_sep_l' -associative -always_and_sep_l'.
+  apply const_elim_l=>-[-> [-> ->]] /=.
+  rewrite -pvs_intro right_id -wp_value.
+  by rewrite wand_elim_r.
+Qed.
+
+
 Lemma wp_load_pst E σ l v Q :
   σ !! l = Some v →
   (ownP σ ★ ▷ (ownP σ -★ Q v)) ⊑ wp E (Load (Loc l)) Q.
 Proof.
-  intros; rewrite -(wp_lift_step E E (λ e' σ', e' = of_val v ∧ σ' = σ)) //;
-    last by intros; inv_step; eauto.
-  rewrite -pvs_intro; apply sep_mono, later_mono; first done.
-  apply forall_intro=>e2; apply forall_intro=>σ2; apply wand_intro_l.
-  rewrite -pvs_intro always_and_sep_l' -associative -always_and_sep_l'.
-  apply const_elim_l=>-[-> ->]; by rewrite wand_elim_r -wp_value.
+  intros; rewrite -(wp_lift_atomic_det_step σ v σ) //;
+    last (by intros; inv_step; eauto).
 Qed.
+
 Lemma wp_store_pst E σ l e v v' Q :
   to_val e = Some v → σ !! l = Some v' →
   (ownP σ ★ ▷ (ownP (<[l:=v]>σ) -★ Q LitUnitV)) ⊑ wp E (Store (Loc l) e) Q.
 Proof.
   intros.
-  rewrite -(wp_lift_step E E (λ e' σ', e' = LitUnit ∧ σ' = <[l:=v]>σ)) //;
+  rewrite -(wp_lift_atomic_det_step σ LitUnitV (<[l:=v]>σ)) //;
     last by intros; inv_step; eauto.
-  rewrite -pvs_intro; apply sep_mono, later_mono; first done.
-  apply forall_intro=>e2; apply forall_intro=>σ2; apply wand_intro_l.
-  rewrite -pvs_intro always_and_sep_l' -associative -always_and_sep_l'.
-  apply const_elim_l=>-[-> ->]; by rewrite wand_elim_r -wp_value'.
 Qed.
+
 Lemma wp_cas_fail_pst E σ l e1 v1 e2 v2 v' Q :
   to_val e1 = Some v1 → to_val e2 = Some v2 → σ !! l = Some v' → v' ≠ v1 →
   (ownP σ ★ ▷ (ownP σ -★ Q LitFalseV)) ⊑ wp E (Cas (Loc l) e1 e2) Q.
 Proof.
-  intros; rewrite -(wp_lift_step E E (λ e' σ', e' = LitFalse ∧ σ' = σ)) //;
+  intros; rewrite -(wp_lift_atomic_det_step σ LitFalseV σ) //;
     last by intros; inv_step; eauto.
-  rewrite -pvs_intro; apply sep_mono, later_mono; first done.
-  apply forall_intro=>e2'; apply forall_intro=>σ2; apply wand_intro_l.
-  rewrite -pvs_intro always_and_sep_l' -associative -always_and_sep_l'.
-  apply const_elim_l=>-[-> ->]; by rewrite wand_elim_r -wp_value'.
 Qed.
+
 Lemma wp_cas_suc_pst E σ l e1 v1 e2 v2 Q :
   to_val e1 = Some v1 → to_val e2 = Some v2 → σ !! l = Some v1 →
   (ownP σ ★ ▷ (ownP (<[l:=v2]>σ) -★ Q LitTrueV)) ⊑ wp E (Cas (Loc l) e1 e2) Q.
 Proof.
   intros.
-  rewrite -(wp_lift_step E E (λ e' σ', e' = LitTrue ∧ σ' = <[l:=v2]>σ)) //;
+  rewrite -(wp_lift_atomic_det_step σ LitTrueV (<[l:=v2]>σ)) //;
     last by intros; inv_step; eauto.
-  rewrite -pvs_intro; apply sep_mono, later_mono; first done.
-  apply forall_intro=>e2'; apply forall_intro=>σ2; apply wand_intro_l.
-  rewrite -pvs_intro always_and_sep_l' -associative -always_and_sep_l'.
-  apply const_elim_l=>-[-> ->]; by rewrite wand_elim_r -wp_value'.
 Qed.
 
 (** Base axioms for core primitives of the language: Stateless reductions *)
@@ -107,6 +99,7 @@ Proof.
   apply sep_intro_True_l; last done.
   by rewrite -wp_value' //; apply const_intro.
 Qed.
+
 Lemma wp_lift_pure_step E (φ : expr → Prop) Q e1 :
   to_val e1 = None →
   (∀ σ1, reducible e1 σ1) →
@@ -118,6 +111,7 @@ Proof.
   apply impl_intro_l, const_elim_l=>-[-> ?] /=.
   by rewrite const_equiv // left_id right_id.
 Qed.
+
 Lemma wp_rec E ef e v Q :
   to_val e = Some v →
   ▷ wp E ef.[Rec ef, e /] Q ⊑ wp E (App (Rec ef) e) Q.
@@ -126,6 +120,7 @@ Proof.
     Q (App (Rec ef) e)) //=; last by intros; inv_step; eauto.
   by apply later_mono, forall_intro=>e2; apply impl_intro_l, const_elim_l=>->.
 Qed.
+
 Lemma wp_plus E n1 n2 Q :
   ▷ Q (LitNatV (n1 + n2)) ⊑ wp E (Plus (LitNat n1) (LitNat n2)) Q.
 Proof.
@@ -134,6 +129,7 @@ Proof.
   apply later_mono, forall_intro=>e2; apply impl_intro_l, const_elim_l=>->.
   by rewrite -wp_value'.
 Qed.
+
 Lemma wp_le_true E n1 n2 Q :
   n1 ≤ n2 →
   ▷ Q LitTrueV ⊑ wp E (Le (LitNat n1) (LitNat n2)) Q.
@@ -143,6 +139,7 @@ Proof.
   apply later_mono, forall_intro=>e2; apply impl_intro_l, const_elim_l=>->.
   by rewrite -wp_value'.
 Qed.
+
 Lemma wp_le_false E n1 n2 Q :
   n1 > n2 →
   ▷ Q LitFalseV ⊑ wp E (Le (LitNat n1) (LitNat n2)) Q.
@@ -152,6 +149,7 @@ Proof.
   apply later_mono, forall_intro=>e2; apply impl_intro_l, const_elim_l=>->.
   by rewrite -wp_value'.
 Qed.
+
 Lemma wp_fst E e1 v1 e2 v2 Q :
   to_val e1 = Some v1 → to_val e2 = Some v2 →
   ▷Q v1 ⊑ wp E (Fst (Pair e1 e2)) Q.
@@ -161,6 +159,7 @@ Proof.
   apply later_mono, forall_intro=>e2'; apply impl_intro_l, const_elim_l=>->.
   by rewrite -wp_value'.
 Qed.
+
 Lemma wp_snd E e1 v1 e2 v2 Q :
   to_val e1 = Some v1 → to_val e2 = Some v2 →
   ▷ Q v2 ⊑ wp E (Snd (Pair e1 e2)) Q.
@@ -170,6 +169,7 @@ Proof.
   apply later_mono, forall_intro=>e2'; apply impl_intro_l, const_elim_l=>->.
   by rewrite -wp_value'.
 Qed.
+
 Lemma wp_case_inl E e0 v0 e1 e2 Q :
   to_val e0 = Some v0 →
   ▷ wp E e1.[e0/] Q ⊑ wp E (Case (InjL e0) e1 e2) Q.
@@ -178,6 +178,7 @@ Proof.
     (Case (InjL e0) e1 e2)) //=; last by intros; inv_step; eauto.
   by apply later_mono, forall_intro=>e1'; apply impl_intro_l, const_elim_l=>->.
 Qed.
+
 Lemma wp_case_inr E e0 v0 e1 e2 Q :
   to_val e0 = Some v0 →
   ▷ wp E e2.[e0/] Q ⊑ wp E (Case (InjR e0) e1 e2) Q.
@@ -197,4 +198,5 @@ Proof.
   * rewrite -wp_le_true; auto.
   * rewrite -wp_le_false; auto with lia.
 Qed.
+
 End lifting.
